

When not otherwise stated,  $\{N(t) : t \geq 0\}$  is a Poisson process with rate  $\lambda > 0$  and event times  $\{T_n : n \geq 1\}$ .

3. Let  $0 < s < t$ .

(a) Find the conditional distribution of  $N(s)$  given  $N(t)$ .

(b) Compute  $E[T_k | N(t)]$  for all  $k \geq 1$ .

$$\begin{aligned}
 a) P(N(s)=k | N(t)=n) &= \frac{P(N(s)=k, N(t)=n)}{P(N(t)=n)} \\
 &= \frac{P(N(s)=k, N(t)-N(s)=n-k)}{P(N(t)=n)} \\
 &= \frac{P(N(s)=k) P(N(t)-N(s)=n-k)}{P(N(t)=n)} \\
 &= \frac{e^{-\lambda s} (\lambda s)^k}{k!} \frac{e^{-\lambda(t-s)} (\lambda(t-s))^{n-k}}{(n-k)!} \frac{n!}{e^{-\lambda t} (\lambda t)^n} \\
 &= \frac{\binom{n}{k} s^k (t-s)^{n-k}}{t^n} \\
 &= \binom{n}{k} \left(\frac{s}{t}\right)^k \left(1 - \frac{s}{t}\right)^{n-k}
 \end{aligned}$$

$$\text{So } \sum_{k=0}^n P(N(s)=k | N(t)=n) = \sum_{k=0}^n \binom{n}{k} \left(\frac{s}{t}\right)^k \left(1 - \frac{s}{t}\right)^{n-k}$$

$$\therefore N(s) | N(t)=n \sim \text{Bin}(n, \frac{s}{t})$$

b) Note  $\{T_n \leq t\} \Leftrightarrow \{N(t) \geq n\}$

$$\begin{aligned}
 P(T_k > s | N(t)=n) &= P(N(s) < k | N(t)=n) \\
 &= \sum_{j=0}^{k-1} \binom{n}{j} \left(\frac{s}{t}\right)^j \left(1 - \frac{s}{t}\right)^{n-j}
 \end{aligned}$$

If  $n < k$ ,  $P(T_k > s | N(t)=n) = P(N(s) < k | N(t)=n) = 0$ .

This is because  $N(u) = \sum_{n=1}^{\infty} 1_{\{T_n \leq u\}}$  so  $N(t)$  cannot equal  $n$  if  $N(s) < k$  and  $s < t$ .

$$\begin{aligned}
 E[T_k | N(t)=n] &= \int_0^{\infty} P(T_k > s | N(t)=n) ds \\
 &= \int_0^{\infty} P(N(s) < k | N(t)=n) ds \\
 &= \int_0^t \sum_{j=0}^{k-1} \binom{n}{j} \left(\frac{s}{t}\right)^j \left(1 - \frac{s}{t}\right)^{n-j} ds \quad \text{because } s < t \\
 &= \sum_{j=0}^{k-1} \binom{n}{j} \int_0^t \left(\frac{s}{t}\right)^j \left(1 - \frac{s}{t}\right)^{n-j} ds \\
 &= \sum_{j=0}^{k-1} \binom{n}{j} \int_0^1 u^j (1-u)^{n-j} \frac{1}{t} du \quad u = \frac{s}{t} \quad du = \frac{1}{t} ds \\
 &= \frac{1}{t} \sum_{j=0}^{k-1} \binom{n}{j} \frac{\Gamma(n-j+1) \Gamma(j+1)}{\Gamma(n-j+j+2)} \quad \text{Beta normalization constant} \\
 &= \frac{1}{t} \sum_{j=0}^{k-1} \frac{n!}{j!(n-j)!} \frac{(n-j)! j!}{(n+1)!} \\
 &= \frac{1}{t} \sum_{j=0}^{k-1} \frac{1}{n+1} \\
 &= \frac{k}{n+1}
 \end{aligned}$$

4. Let  $\{M(t) : t \geq 0\}$  be a Poisson process with rate  $\mu$  and event times  $\{S_n : n \geq 1\}$  independent of  $\{N(t)\}$  and  $\{T_n\}$ . Determine if the process  $\{L(t) : t \geq 0\}$  is a Poisson process, and if so compute its rate.

(a)  $L(t) = N(t) + M(t)$ .

(b)  $L(t)$  is the counting process on  $[0, \infty)$  with event times  $R_n = \min\{S_n, T_n\}$ ,  $n \geq 1$ .

(c)  $L(t)$  counts the number of intervals  $(k-1, k]$ ,  $k = 1, 2, \dots, N(t)$  for which  $M(k-1, k] = 0$ , i.e., on which the process  $\{M(t)\}$  sees no events.

a)  $L(0) = N(0) + M(0) = 0$

$L(t) - L(s) = N(t) + M(t) - (N(s) + M(s))$

$= N(t) - N(s) + M(t) - M(s)$

So  $L$  has stationary increments

$G_{N(t)}(s) = \sum_{k=0}^{\infty} s^k \frac{e^{-\lambda} \lambda^k}{k!} = e^{-\lambda} e^{s\lambda} = e^{\lambda(s-1)}$

$G_{M(t)}(s) = e^{\mu(s-1)}$

$G_{N(t)}(s)G_{M(t)}(s) = e^{\lambda(s-1)} e^{\mu(s-1)} = e^{(\lambda+\mu)(s-1)} = G_{N(t)+M(t)}(s) = G_{L(t)}(s)$

Thus the rate is  $\lambda + \mu$

b)  $L(t) = \sum_{n=1}^{\infty} \mathbb{I}\{\min(T_n, S_n) \leq t\}$

$L(0) = \sum_{n=1}^{\infty} \mathbb{I}\{\min(T_n, S_n) \leq 0\} = 0$  since  $T_n, S_n \geq 0$

WLOG assume  $T_n = \min(T_n, S_n)$

$L(t) - L(s) = \sum_{n=1}^{\infty} \mathbb{I}\{T_n \leq t\} - \mathbb{I}\{T_n \leq s\}$   
 $= N(t) - N(s)$

Thus  $L$  has stationary increments

$R_n = \min\{T_n, S_n\}$

$P(R_n \leq x) = 1 - P(R_n > x)$   
 $= 1 - P(T_n > x)P(S_n > x)$   
 $= 1 - e^{-(\lambda+\mu)x}$

Thus the rate is  $\lambda + \mu$

c) From class  $L(t) = \sum_{k=1}^{N(t)} \mathbb{I}\{M(k-1, k] = 0\}$

$\mathbb{I}\{M(k-1, k] = 0\} \sim \text{Ber}(e^{-\mu})$

It follows  $L(t) | N(t) = n \sim \text{Bin}(n, e^{-\mu})$

$P(L(t) = m) = \sum_{n=0}^{\infty} P(L(t) = m | N(t) = n) P(N(t) = n)$

$= \sum_{n=m}^{\infty} \binom{n}{m} e^{-\mu m} (1 - e^{-\mu})^{n-m} \frac{e^{-\lambda} \lambda^n}{n!}$

Because  $\text{Bin}(n, e^{-\mu}) = 0$  for  $n < m$

$= \frac{e^{-\lambda} \lambda^m}{m!} \sum_{n=m}^{\infty} \frac{\lambda^{n-m}}{(n-m)!} (1 - e^{-\mu})^{n-m} \frac{(\lambda + \mu)^m}{(\lambda + \mu)^m}$

$= \frac{e^{-\lambda} (e^{-\mu} \lambda)^m}{m!} \sum_{k=0}^{\infty} \frac{(\lambda + (1 - e^{-\mu}))^k}{k!}$

$= e^{-\lambda} e^{\lambda(1-e^{-\mu})} \frac{(e^{-\mu} \lambda)^m}{m!}$

$= e^{-\mu \lambda t} e^{-\lambda t} \frac{(e^{-\mu} \lambda)^m}{m!}$

$$= e^{-\mu} e^{-\mu t} \frac{(e^{-\mu} \lambda t)^m}{m!}$$

$$= \frac{(e^{-\mu} \lambda t)^m}{m!} e^{-\mu} e^{-\mu t}$$

Thus  $L(t) \sim \text{Poisson}(e^{-\mu} \lambda t) \Rightarrow$  rate of  $L$  is  $e^{-\mu} \lambda$

- $L(0) = 0$

- Since  $L(t) \sim \text{Poisson}(e^{-\mu} \lambda t)$

$$L(t) - L(s) = L(t-s)$$